

1. Solve for \( x \):
   \[
   4x - 7 = 3x + 5
   \]

2. Solve for \( y \) in terms of \( x \):
   \[
   2y - 3x = 7
   \]

3. Solve for \( z \):
   \[
   5(z - 2) + 3 = 4z + 8
   \]

4. Solve for \( a \) in terms of \( b \):
   \[
   6a + 2b = 3a - 5b + 14
   \]

5. Solve for \( t \):
   \[
   3(2t + 5) = 7(t - 1) - 2
   \]

6. Solve for \( k \) in terms of \( m \):
   \[
   8k - 3m = 2(k + 4m) + 10
   \]

7. Solve for \( n \):
   \[
   \frac{n - 2}{3} + \frac{n + 4}{2} = 5
   \]

8. Solve for \( x \) in terms of \( y \):
   \[
   \frac{3x - y}{2} = \frac{2x + y}{4}
   \]

9. Solve for \( p \):
   \[
   4p + 7 - 3p = 2p + 10 - p
   \]

10. Solve for \( b \) in terms of \( a \):
    \[
    \frac{b - 4}{a} + 3 = \frac{b + 2}{2a}
    \]

## Simplifying expressions by distributing and combining like terms.

### Example of simplify the given expression: 
### \(-7q^2(4q^3 - 9q^2 + q - 3)\), 
### follow these steps:


1. **Distribute \(-7q^2\) to each term inside the parentheses:**

\[
-7q^2(4q^3) - 7q^2(-9q^2) + -7q^2(q) + -7q^2(-3)
\]

2. **Simplify each term:**

- First term: \(-7q^2 \cdot 4q^3\)
  \[
  -7 \cdot 4 \cdot q^2 \cdot q^3 = -28q^{2+3} = -28q^5
  \]

- Second term: \(-7q^2 \cdot (-9q^2)\)
  \[
  -7 \cdot (-9) \cdot q^2 \cdot q^2 = 63q^{2+2} = 63q^4
  \]

- Third term: \(-7q^2 \cdot q\)
  \[
  -7 \cdot q^2 \cdot q = -7q^{2+1} = -7q^3
  \]

- Fourth term: \(-7q^2 \cdot (-3)\)
  \[
  -7 \cdot (-3) \cdot q^2 = 21q^2
  \]

3. **Combine all the simplified terms:**

\[
-28q^5 + 63q^4 - 7q^3 + 21q^2
\]

So, the simplified expression is:

\[
-28q^5 + 63q^4 - 7q^3 + 21q^2
\]


### Simplifying expressions of following


1. Simplify:
   \[
   3x^2(2x^3 - 4x^2 + 5x - 7)
   \]

2. Simplify:
   \[
   -5y^2(3y^3 + 6y^2 - 2y + 4)
   \]

3. Simplify:
   \[
   4z^2(5z^3 - z^2 + 2z - 3)
   \]

4. Simplify:
   \[
   -2a^3(4a^3 - 3a^2 + a - 5)
   \]

5. Simplify:
   \[
   7b^2(6b^3 - 2b^2 + 3b - 4)
   \]

 